frame definitions and axioms

FrameTheory/Frame.lean
@@ -4,24 +4,82 @@ Author: Tally Holcombe
 -/
 import Mathlib.Order.CompleteLattice
 import Mathlib.Order.Lattice
+import Mathlib.Order.BoundedOrder
 
 
-class Frame (α : Type u) extends CompleteLattice α, DistribLattice α where
-  inf_sup_le_sup_inf : ∀ (S: Set α) (a: α), a ⊓ sSup S = sSup { a ⊓ s | s ∈ S} -- infinite distributive law
+-- class Frame (α : Type u) extends CompleteLattice α where
+--   inf_sup_le_sup_inf : ∀ (S: Set α) (a: α), a ⊓ sSup S = sSup { a ⊓ s | s ∈ S} -- frame distributive law
+
+
+-- open Frame
+
+-- variable {α : Type u} [Frame α]
+
+-- theorem Frame.sup_lub (x : α) (S : Set α) (h : ∀ y ∈ S, y ≤ x) : sSup S ≤ x := by
+--   have h2 := CompleteLattice.sSup_le S x h
+--   exact h2
+
+
+-- lemma Frame.sup_refl (x : α) : x ⊔ x = x := by
+--   exact sup_idem x
+
+-- lemma Frame.sup_associative ( x y z : α) : x ⊔ y ⊔ z = x ⊔ (y ⊔ z) := by
+--   exact sup_assoc x y z
+
+-- lemma Frame.sup_commutative (x y : α) : x ⊔ y = y ⊔ x := by
+--   exact sup_comm x y
+
+-- lemma Frame.absorb_join (x y : α) : x ⊔ (x ⊓ y) = x := by
+--   exact sup_inf_self
+
+-- lemma Frame.absorb_meet (x y : α) : x ⊓ (x ⊔ y) = x := by
+--   exact inf_sup_self
+
+-- lemma Frame.left_meet_distributive (x y z : α) : x ⊓ (y ⊔ z) = (x ⊓ y) ⊔ (x ⊓ z) := by
+--   exact inf_sup_left x y z
+
+
+
+class Frame (α : Type u) extends CompleteSemilatticeSup α, SemilatticeInf α, BoundedOrder α, Lattice α where
+  inf_sup_le_sup : ∀ (a : α) (S : Set α), inf a (sSup S) = sSup {inf a s | s ∈ S} -- = or ≤ ?
+  protected leq_sup_inf : ∀ x y z : α, inf (sup x  y) (sup x  z) ≤ sup x (inf y z)     -- trait from DistribLattice
+  protected leq_inf_sup : ∀ x y z : α, sup (inf x y) (inf x z) ≤ inf x (sup y z)
+
+  protected sup_inf_leq : ∀ x y z : α, sup x (inf y z) ≤ inf (sup x y) (sup x z)
+  protected inf_sup_leq : ∀ x y z : α, inf x (sup y z) ≤ sup (inf x y) (inf x z)
 
 
 open Frame
 
 variable {α : Type u} [Frame α]
 
+theorem leq_sup_inf (x y z : α) : (x ⊔ y) ⊓ (x ⊔ z) ≤ x ⊔ (y ⊓ z) := by
+  exact Frame.leq_sup_inf x y z
+
+theorem leq_inf_sup (x y z : α) : (x ⊓ y) ⊔ (x ⊓ z) ≤ x ⊓ (y ⊔ z) := by
+  exact Frame.leq_inf_sup x y z
+
+
+theorem sup_inf_leq (x y z : α) : x ⊔ (y ⊓ z) ≤ (x ⊔ y) ⊓ (x ⊔ z) := by
+  exact Frame.sup_inf_leq x y z
+
+theorem inf_sup_leq (x y z : α) : x ⊓ (y ⊔ z) ≤ (x ⊓ y) ⊔ (x ⊓ z) := by
+  exact Frame.inf_sup_leq x y z
+
+
+-- join-distributive
+theorem Frame.sup_inf_left (x y z : α) : x ⊔ (y ⊓ z) = (x ⊔ y) ⊓ (x ⊔ z) :=
+  le_antisymm (sup_inf_leq x y z) (leq_sup_inf x y z)
+
+-- meet-distributive
+theorem Frame.inf_sup_left (x y z : α) : x ⊓ (y ⊔ z) = (x ⊓ y) ⊔ (x ⊓ z) :=
+  le_antisymm (inf_sup_leq x y z) (leq_inf_sup x y z)
+
+-- LUB
 theorem Frame.sup_lub (x : α) (S : Set α) (h : ∀ y ∈ S, y ≤ x) : sSup S ≤ x := by
-  have h2 := CompleteLattice.sSup_le S x h
-  exact h2
+  exact CompleteSemilatticeSup.sSup_le S x h
 
-
-
-
-
+-- axioms
 lemma Frame.sup_refl (x : α) : x ⊔ x = x := by
   exact sup_idem x
 
@@ -36,6 +94,3 @@ lemma Frame.absorb_join (x y : α) : x ⊔ (x ⊓ y) = x := by
 
 lemma Frame.absorb_meet (x y : α) : x ⊓ (x ⊔ y) = x := by
   exact inf_sup_self
-
-lemma Frame.left_meet_distributive (x y z : α) : x ⊓ (y ⊔ z) = (x ⊓ y) ⊔ (x ⊓ z) := by
-  exact inf_sup_left x y z
